scheduler/SchIAproof.v
@@ -9,9 +9,9 @@ Local Open Scope nat_scope.
 
 Module SchIA. Section SchIA.
   Import SchAS.
-  Context `{!invG α Σ Γ, !subG Γ Σ, !sinvG Σ Γ α β τ, !SchAGΣ Σ, !SchAGΓ Γ}.
-  Context (u_a : univ_id).
+  Context `{!sinvG Γ Σ α β τ, !schG Γ Σ α β τ}.
 
+  Context (u_a : univ_id).
   Context (Sp_global Sp_user : string -> option fspec).
   Context (SchInSp : sp_incl (sp u_a Sp_user) Sp_global).
   Context (FunInSp : sp_sub Sp_user Sp_global).
@@ -171,7 +171,7 @@ Module SchIA. Section SchIA.
   Local Definition SchIMod := (SchI.t).
 
   Lemma simF__spawn : HSim.sim_fun open SchAMod SchIMod Ist SchHdr._spawn.
-  Proof using sinvG0 FunInSp SchInSp.
+  Proof using FunInSp SchInSp.
     init_simF u_a 0.
 
     rewrite /SchA.trigger_Yield /SchI.trigger_Yield.
@@ -339,7 +339,7 @@ Module SchIA. Section SchIA.
   (*FAST*)Qed.
 
   Lemma simF_spawn : HSim.sim_fun open SchAMod SchIMod Ist SchHdr.spawn.
-  Proof using sinvG0 FunInSp SchInSp.
+  Proof using FunInSp SchInSp.
     init_simF u_a 0.
 
     step_l. step_l. destruct q as [[[[farg fvarg] pre] synpost] userf].
@@ -408,7 +408,7 @@ Module SchIA. Section SchIA.
   (*FAST*)Qed.
 
   Lemma simF_yield : HSim.sim_fun open SchAMod SchIMod Ist SchHdr.yield.
-  Proof using sinvG0 FunInSp SchInSp.
+  Proof using FunInSp SchInSp.
     init_simF u_a 0.
 
     rewrite /SchA.trigger_Yield /SchI.trigger_Yield.
@@ -441,7 +441,7 @@ Module SchIA. Section SchIA.
   (*FAST*)Qed.
 
   Lemma simF_join : HSim.sim_fun open SchAMod SchIMod Ist SchHdr.join.
-  Proof using sinvG0 FunInSp SchInSp.
+  Proof using FunInSp SchInSp.
     init_simF u_a 0.
 
     step_l. step_l.
@@ -540,7 +540,7 @@ Module SchIA. Section SchIA.
   (*FAST*)Qed.
 
   Lemma simF_get_tid : HSim.sim_fun open SchAMod SchIMod Ist SchHdr.get_tid.
-  Proof using sinvG0 FunInSp SchInSp.
+  Proof using FunInSp SchInSp.
     init_simF u_a 0.
 
     steps_l. iDestruct "ASM" as "[[-> tid] ->]"; hss.
@@ -553,7 +553,7 @@ Module SchIA. Section SchIA.
   (*FAST*)Qed.
 
   Lemma sim : HSim.t open SchAMod SchIMod SchA.init_cond Ist.
-  Proof using sinvG0 FunInSp SchInSp.
+  Proof using FunInSp SchInSp.
     init_sim.
     - rewrite /SchA.init_cond /init_threads /init_tid. unseal "SchA".
       iIntros "[[THB THW] tid]". iExists _, _, _, ∅, 0, false.
@@ -580,8 +580,7 @@ Module SchIA. Section SchIA.
   End SchIA.
 
   Section ctxr.
-    Context `{!invG α Σ Γ, !subG Γ Σ, !sinvG Σ Γ α β τ}.
-    Context `{!SchAGΣ Σ, !SchAGΓ Γ}.
+    Context `{!sinvG Γ Σ α β τ, !schG Γ Σ α β τ}.
     Lemma ctxr (u : univ_id) (sp_global sp_user : string → option fspec)
         (SchInGlobal : sp_incl (SchAS.sp u sp_user) sp_global)
         (UserInGlobal : sp_sub sp_user sp_global) :
